common/Events.v
@@ -626,7 +626,7 @@ in extcall_caller_independent.
 *)
 
 Definition extcall_sem : Type :=
-  Senv.t -> list val -> mem -> trace -> val -> mem -> Prop.
+  Senv.t -> compartment -> list val -> mem -> trace -> val -> mem -> Prop.
 
 (* (** This invariant guarantees that external calls performed to [cp] can *)
 (*   correctly use either [cp1] or [cp2] to find out who the calling compartment *)
@@ -670,21 +670,21 @@ Record extcall_properties (sem: extcall_sem) (cp: compartment) (sg: signature) :
 (** The return value of an external call must agree with its signature. *)
   ec_well_typed:
     forall ge vargs m1 t vres m2,
-    sem ge vargs m1 t vres m2 ->
+    sem ge cp vargs m1 t vres m2 ->
     Val.has_rettype vres sg.(sig_res);
 
 (** The semantics is invariant under change of global environment that preserves symbols. *)
   ec_symbols_preserved:
     forall ge1 ge2 vargs m1 t vres m2,
     Senv.equiv ge1 ge2 ->
-    sem ge1 vargs m1 t vres m2 ->
-    sem ge2 vargs m1 t vres m2;
+    sem ge1 cp vargs m1 t vres m2 ->
+    sem ge2 cp vargs m1 t vres m2;
 
 (** External calls cannot invalidate memory blocks.  (Remember that
   freeing a block does not invalidate its block identifier.) *)
   ec_valid_block:
     forall ge vargs m1 t vres m2 b,
-    sem ge vargs m1 t vres m2 ->
+    sem ge cp vargs m1 t vres m2 ->
     Mem.valid_block m1 b -> Mem.valid_block m2 b;
 
 (** External calls cannot change the ownership of memory blocks.
@@ -692,50 +692,51 @@ Record extcall_properties (sem: extcall_sem) (cp: compartment) (sg: signature) :
       notion of [can_access_block] must be completely changed anyway
  *)
   ec_can_access_block:
-    forall ge vargs m1 t vres m2 b cp,
-    sem ge vargs m1 t vres m2 ->
-    Mem.can_access_block m1 b cp -> Mem.can_access_block m2 b cp;
+    forall ge vargs m1 t vres m2 b ocp,
+    sem ge cp vargs m1 t vres m2 ->
+    Mem.can_access_block m1 b ocp -> Mem.can_access_block m2 b ocp;
 
 (** External calls cannot increase the max permissions of a valid block.
     They can decrease the max permissions, e.g. by freeing. *)
   ec_max_perm:
     forall ge vargs m1 t vres m2 b ofs p,
-    sem ge vargs m1 t vres m2 ->
+    sem ge cp vargs m1 t vres m2 ->
     Mem.valid_block m1 b -> Mem.perm m2 b ofs Max p -> Mem.perm m1 b ofs Max p;
 
 (** External call cannot modify memory unless they have [Max, Writable]
    permissions. *)
   ec_readonly:
-    forall ge vargs m1 t vres m2 b ofs n bytes cp,
-    sem ge vargs m1 t vres m2 ->
+    forall ge vargs m1 t vres m2 b ofs n bytes ocp,
+    sem ge cp vargs m1 t vres m2 ->
     Mem.valid_block m1 b ->
-    Mem.loadbytes m2 b ofs n cp = Some bytes ->
+    Mem.loadbytes m2 b ofs n ocp = Some bytes ->
     (forall i, ofs <= i < ofs + n -> ~Mem.perm m1 b i Max Writable) ->
-    Mem.loadbytes m1 b ofs n cp = Some bytes;
+    Mem.loadbytes m1 b ofs n ocp = Some bytes;
 
 (** External call can only allocate in the calling compartment *)
   ec_new_valid:
     forall ge vargs m1 t vres m2 b,
-    sem ge vargs m1 t vres m2 ->
+    sem ge cp vargs m1 t vres m2 ->
     ~ Mem.valid_block m1 b ->
     Mem.valid_block m2 b ->
     Mem.block_compartment m2 b = Some cp;
 
 (** TODO: External call should not be able to modify other compartment's memory *)
+(** TODO: Is this an acceptable axiom? *)
   ec_mem_outside_compartment:
     forall ge vargs m1 t vres m2,
-    sem ge vargs m1 t vres m2 ->
+    sem ge cp vargs m1 t vres m2 ->
     Mem.unchanged_on (loc_not_in_compartment cp m1) m1 m2;
 
 (** External calls must commute with memory extensions, in the
   following sense. *)
   ec_mem_extends:
     forall ge vargs m1 t vres m2 m1' vargs',
-    sem ge vargs m1 t vres m2 ->
+    sem ge cp vargs m1 t vres m2 ->
     Mem.extends m1 m1' ->
     Val.lessdef_list vargs vargs' ->
     exists vres', exists m2',
-       sem ge vargs' m1' t vres' m2'
+       sem ge cp vargs' m1' t vres' m2'
     /\ Val.lessdef vres vres'
     /\ Mem.extends m2 m2'
     /\ Mem.unchanged_on (loc_out_of_bounds m1) m1' m2';
@@ -745,18 +746,18 @@ Record extcall_properties (sem: extcall_sem) (cp: compartment) (sg: signature) :
   ec_mem_inject:
     forall ge1 ge2 vargs m1 t vres m2 f m1' vargs',
     symbols_inject f ge1 ge2 ->
-    sem ge1 vargs m1 t vres m2 ->
+    sem ge1 cp vargs m1 t vres m2 ->
     Mem.inject f m1 m1' ->
     Val.inject_list f vargs vargs' ->
     exists f', exists vres', exists m2',
-       sem ge2 vargs' m1' t vres' m2'
+       sem ge2 cp vargs' m1' t vres' m2'
     /\ Val.inject f' vres vres'
     /\ Mem.inject f' m2 m2'
     /\ Mem.unchanged_on (loc_unmapped f) m1 m2
     /\ Mem.unchanged_on (loc_out_of_reach f m1) m1' m2'
     /\ inject_incr f f'
     /\ inject_separated f f' m1 m1' /\
-         (* TODO: redundancy with [ec_new_valid]? *)
+         (* TODO: is this a redundancy with [ec_new_valid]? *)
          (forall b,
     ~ Mem.valid_block m1 b ->
     Mem.valid_block m2 b ->
@@ -766,24 +767,24 @@ Record extcall_properties (sem: extcall_sem) (cp: compartment) (sg: signature) :
 (** External calls produce at most one event. *)
   ec_trace_length:
     forall ge vargs m t vres m',
-    sem ge vargs m t vres m' -> (length t <= 1)%nat;
+    sem ge cp vargs m t vres m' -> (length t <= 1)%nat;
 
 (** External calls must be receptive to changes of traces by another, matching trace. *)
   ec_receptive:
     forall ge vargs m t1 vres1 m1 t2,
-    sem ge vargs m t1 vres1 m1 -> match_traces ge t1 t2 ->
-    exists vres2, exists m2, sem ge vargs m t2 vres2 m2;
+    sem ge cp vargs m t1 vres1 m1 -> match_traces ge t1 t2 ->
+    exists vres2, exists m2, sem ge cp vargs m t2 vres2 m2;
 
 (** External calls must be deterministic up to matching between traces. *)
   ec_determ:
     forall ge vargs m t1 vres1 m1 t2 vres2 m2,
-    sem ge vargs m t1 vres1 m1 -> sem ge vargs m t2 vres2 m2 ->
+    sem ge cp vargs m t1 vres1 m1 -> sem ge cp vargs m t2 vres2 m2 ->
     match_traces ge t1 t2 /\ (t1 = t2 -> vres1 = vres2 /\ m1 = m2);
 
 (** External calls cannot produce [Event_call] or [Event_return] events *)
   ec_no_crossing:
     forall ge vargs m t vres m',
-    sem ge vargs m t vres m' ->
+    sem ge cp vargs m t vres m' ->
     match t with
     | Event_call _ _ _ _ :: _
     | Event_return _ _ _ :: _ => False
@@ -793,11 +794,11 @@ Record extcall_properties (sem: extcall_sem) (cp: compartment) (sg: signature) :
 
 (** ** Semantics of volatile loads *)
 
-Inductive volatile_load_sem (cp: compartment) (chunk: memory_chunk) (ge: Senv.t) :
+Inductive volatile_load_sem (chunk: memory_chunk) (ge: Senv.t) (cp: compartment) :
               list val -> mem -> trace -> val -> mem -> Prop :=
   | volatile_load_sem_intro: forall b ofs m t v,
       volatile_load ge cp chunk m b ofs t v ->
-      volatile_load_sem cp chunk ge (Vptr b ofs :: nil) m t v m.
+      volatile_load_sem chunk ge cp (Vptr b ofs :: nil) m t v m.
 
 Lemma volatile_load_preserved:
   forall ge1 ge2 cp chunk m b ofs t v,
@@ -866,7 +867,7 @@ Qed.
 
 Lemma volatile_load_ok:
   forall chunk cp,
-  extcall_properties (volatile_load_sem cp chunk)
+  extcall_properties (volatile_load_sem chunk)
                      cp (mksignature (Tptr :: nil) (rettype_of_chunk chunk) cc_default).
 Proof.
   intros; constructor; intros.
@@ -920,11 +921,11 @@ Qed.
 
 (* JT: Note: Same remarks as for volatile loads *)
 
-Inductive volatile_store_sem (cp: compartment) (chunk: memory_chunk)(ge: Senv.t):
+Inductive volatile_store_sem (chunk: memory_chunk) (ge: Senv.t) (cp: compartment):
               list val -> mem -> trace -> val -> mem -> Prop :=
   | volatile_store_sem_intro: forall b ofs m1 v t m2,
       volatile_store ge cp chunk m1 b ofs v t m2 ->
-      volatile_store_sem cp chunk ge (Vptr b ofs :: v :: nil) m1 t Vundef m2.
+      volatile_store_sem chunk ge cp (Vptr b ofs :: v :: nil) m1 t Vundef m2.
 
 Lemma volatile_store_preserved:
   forall ge1 ge2 cp chunk m1 b ofs v t m2,
@@ -1044,7 +1045,7 @@ Qed.
 
 Lemma volatile_store_ok:
   forall cp chunk,
-  extcall_properties (volatile_store_sem cp chunk)
+  extcall_properties (volatile_store_sem chunk)
                      cp (mksignature (Tptr :: type_of_chunk chunk :: nil) Tvoid cc_default).
 Proof.
   intros; constructor; intros.
@@ -1094,16 +1095,16 @@ Qed.
 
 (* JT: NOTE: Same remarks as for volatile loads and stores *)
 
-Inductive extcall_malloc_sem (cp: compartment) (ge: Senv.t):
+Inductive extcall_malloc_sem (ge: Senv.t) (cp: compartment):
               list val -> mem -> trace -> val -> mem -> Prop :=
   | extcall_malloc_sem_intro: forall sz m m' b m'',
       Mem.alloc m cp (- size_chunk Mptr) (Ptrofs.unsigned sz) = (m', b) ->
       Mem.store Mptr m' b (- size_chunk Mptr) (Vptrofs sz) cp = Some m'' ->
-      extcall_malloc_sem cp ge (Vptrofs sz :: nil) m E0 (Vptr b Ptrofs.zero) m''.
+      extcall_malloc_sem ge cp (Vptrofs sz :: nil) m E0 (Vptr b Ptrofs.zero) m''.
 
 Lemma extcall_malloc_ok:
   forall cp,
-  extcall_properties (extcall_malloc_sem cp)
+  extcall_properties (extcall_malloc_sem)
                      cp (mksignature (Tptr :: nil) Tptr cc_default).
 Proof.
   intros.
@@ -1204,19 +1205,19 @@ Qed.
 
 (* JT: NOTE: Same remarks as before. *)
 
-Inductive extcall_free_sem (cp: compartment) (ge: Senv.t):
+Inductive extcall_free_sem (ge: Senv.t) (cp: compartment):
               list val -> mem -> trace -> val -> mem -> Prop :=
   | extcall_free_sem_ptr: forall b lo sz m m',
       Mem.load Mptr m b (Ptrofs.unsigned lo - size_chunk Mptr) (Some cp) = Some (Vptrofs sz) ->
       Ptrofs.unsigned sz > 0 ->
       Mem.free m b (Ptrofs.unsigned lo - size_chunk Mptr) (Ptrofs.unsigned lo + Ptrofs.unsigned sz) cp = Some m' ->
-      extcall_free_sem cp ge (Vptr b lo :: nil) m E0 Vundef m'
+      extcall_free_sem ge cp (Vptr b lo :: nil) m E0 Vundef m'
   | extcall_free_sem_null: forall m,
-      extcall_free_sem cp ge (Vnullptr :: nil) m E0 Vundef m.
+      extcall_free_sem ge cp (Vnullptr :: nil) m E0 Vundef m.
 
 Lemma extcall_free_ok:
   forall cp,
-  extcall_properties (extcall_free_sem cp)
+  extcall_properties extcall_free_sem
                      cp (mksignature (Tptr :: nil) Tvoid cc_default).
 Proof.
   intros.
@@ -1329,7 +1330,7 @@ Qed.
 (* RB: NOTE: This operation seems particularly interesting in the sense that it
    copies between two blocks, and their respective ownerships must agree. *)
 
-Inductive extcall_memcpy_sem (cp: compartment) (sz al: Z) (ge: Senv.t):
+Inductive extcall_memcpy_sem (sz al: Z) (ge: Senv.t) (cp: compartment):
                         list val -> mem -> trace -> val -> mem -> Prop :=
   | extcall_memcpy_sem_intro: forall bdst odst bsrc osrc m bytes m',
       al = 1 \/ al = 2 \/ al = 4 \/ al = 8 -> sz >= 0 -> (al | sz) ->
@@ -1340,11 +1341,11 @@ Inductive extcall_memcpy_sem (cp: compartment) (sz al: Z) (ge: Senv.t):
                    \/ Ptrofs.unsigned odst + sz <= Ptrofs.unsigned osrc ->
       Mem.loadbytes m bsrc (Ptrofs.unsigned osrc) sz (Some cp) = Some bytes ->
       Mem.storebytes m bdst (Ptrofs.unsigned odst) bytes cp = Some m' ->
-      extcall_memcpy_sem cp sz al ge (Vptr bdst odst :: Vptr bsrc osrc :: nil) m E0 Vundef m'.
+      extcall_memcpy_sem sz al ge cp (Vptr bdst odst :: Vptr bsrc osrc :: nil) m E0 Vundef m'.
 
 Lemma extcall_memcpy_ok:
   forall cp sz al,
-  extcall_properties (extcall_memcpy_sem cp sz al)
+  extcall_properties (extcall_memcpy_sem sz al)
                      cp (mksignature (Tptr :: Tptr :: nil) Tvoid cc_default).
 Proof.
   intros. constructor.
@@ -1474,15 +1475,15 @@ Qed.
 
 (* JT: NOTE: Same as before *)
 
-Inductive extcall_annot_sem (cp: compartment) (text: string) (targs: list typ) (ge: Senv.t):
+Inductive extcall_annot_sem (text: string) (targs: list typ) (ge: Senv.t) (cp: compartment):
               list val -> mem -> trace -> val -> mem -> Prop :=
   | extcall_annot_sem_intro: forall vargs m args,
       eventval_list_match ge args targs vargs ->
-      extcall_annot_sem cp text targs ge vargs m (Event_annot text args :: E0) Vundef m.
+      extcall_annot_sem text targs ge cp vargs m (Event_annot text args :: E0) Vundef m.
 
 Lemma extcall_annot_ok:
   forall cp text targs,
-  extcall_properties (extcall_annot_sem cp text targs)
+  extcall_properties (extcall_annot_sem text targs)
                      cp (mksignature targs Tvoid cc_default).
 Proof.
   intros; constructor; intros.
@@ -1528,15 +1529,15 @@ Proof.
 - inv H; simpl; auto.
 Qed.
 
-Inductive extcall_annot_val_sem (cp: compartment) (text: string) (targ: typ) (ge: Senv.t):
+Inductive extcall_annot_val_sem (text: string) (targ: typ) (ge: Senv.t) (cp: compartment):
               list val -> mem -> trace -> val -> mem -> Prop :=
   | extcall_annot_val_sem_intro: forall varg m arg,
       eventval_match ge arg targ varg ->
-      extcall_annot_val_sem cp text targ ge (varg :: nil) m (Event_annot text (arg :: nil) :: E0) varg m.
+      extcall_annot_val_sem text targ ge cp (varg :: nil) m (Event_annot text (arg :: nil) :: E0) varg m.
 
 Lemma extcall_annot_val_ok:
   forall cp text targ,
-  extcall_properties (extcall_annot_val_sem cp text targ)
+  extcall_properties (extcall_annot_val_sem text targ)
                      cp (mksignature (targ :: nil) targ cc_default).
 Proof.
   intros; constructor; intros.
@@ -1582,14 +1583,14 @@ Proof.
 - inv H; simpl; auto.
 Qed.
 
-Inductive extcall_debug_sem (cp: compartment) (ge: Senv.t):
+Inductive extcall_debug_sem (ge: Senv.t) (cp: compartment):
               list val -> mem -> trace -> val -> mem -> Prop :=
   | extcall_debug_sem_intro: forall vargs m,
-      extcall_debug_sem cp ge vargs m E0 Vundef m.
+      extcall_debug_sem ge cp vargs m E0 Vundef m.
 
 Lemma extcall_debug_ok:
   forall cp targs,
-  extcall_properties (extcall_debug_sem cp)
+  extcall_properties extcall_debug_sem
                      cp (mksignature targs Tvoid cc_default).
 Proof.
   intros; constructor; intros.
@@ -1640,11 +1641,11 @@ Qed.
   as defined in the [Builtin] modules.
   These built-in functions have no observable effects and do not access memory. *)
 
-Inductive known_builtin_sem (bf: builtin_function) (ge: Senv.t):
+Inductive known_builtin_sem (bf: builtin_function) (ge: Senv.t) (cp: compartment):
               list val -> mem -> trace -> val -> mem -> Prop :=
   | known_builtin_sem_intro: forall vargs vres m,
       builtin_function_sem bf vargs = Some vres ->
-      known_builtin_sem bf ge vargs m E0 vres m.
+      known_builtin_sem bf ge cp vargs m E0 vres m.
 
 Lemma known_builtin_ok: forall bf cp,
   extcall_properties (known_builtin_sem bf) cp (builtin_function_sig bf).
@@ -1706,55 +1707,35 @@ Qed.
   are not described in [Builtins].
 *)
 
-Parameter external_functions_sem: compartment -> String.string -> signature -> extcall_sem.
+Parameter external_functions_sem: String.string -> signature -> extcall_sem.
 
 Axiom external_functions_properties:
-  forall id sg cp, extcall_properties (external_functions_sem cp id sg) cp sg.
-
-(* Axiom external_functions_caller_independent: *)
-(*   forall cp id sg, extcall_caller_independent cp (external_functions_sem id sg). *)
-(* Hint Resolve external_functions_caller_independent : caller_independent. *)
+  forall id sg cp, extcall_properties (external_functions_sem id sg) cp sg.
 
 (** We treat inline assembly similarly. *)
 
-Parameter inline_assembly_sem: compartment -> String.string -> signature -> extcall_sem.
+Parameter inline_assembly_sem: String.string -> signature -> extcall_sem.
 
 Axiom inline_assembly_properties:
-  forall cp id sg, extcall_properties (inline_assembly_sem cp id sg) cp sg.
-
-(* Axiom inline_assembly_caller_independent: *)
-(*   forall cp id sg, extcall_caller_independent cp (inline_assembly_sem id sg). *)
-(* Hint Resolve inline_assembly_caller_independent : caller_independent. *)
+  forall cp id sg, extcall_properties (inline_assembly_sem id sg) cp sg.
 
 (** ** Combined semantics of external calls *)
 
-Definition builtin_or_external_sem name cp sg :=
-  match lookup_builtin_function name cp sg with
+Definition builtin_or_external_sem name sg :=
+  match lookup_builtin_function name sg with
   | Some bf => known_builtin_sem bf
-  | None => external_functions_sem cp name sg
+  | None => external_functions_sem name sg
   end.
 
-Lemma builtin_or_external_sem_ok: forall name sg cp,
-  extcall_properties (builtin_or_external_sem name cp sg) cp sg.
+Lemma builtin_or_external_sem_ok: forall cp name sg,
+  extcall_properties (builtin_or_external_sem name sg) cp sg.
 Proof.
   unfold builtin_or_external_sem; intros. 
-  destruct (lookup_builtin_function name cp sg) as [bf|] eqn:L.
+  destruct (lookup_builtin_function name sg) as [bf|] eqn:L.
 - exploit lookup_builtin_function_sig; eauto. intros EQ; subst sg.
   apply known_builtin_ok.
 - apply external_functions_properties.
 Qed.
-
-(* Lemma builtin_or_external_caller_independent: *)
-(*   forall cp name sg, *)
-(*   extcall_caller_independent cp (builtin_or_external_sem name sg). *)
-(* Proof. *)
-(*   unfold builtin_or_external_sem. *)
-(*   intros cp name sg. *)
-(*   destruct (lookup_builtin_function name sg). *)
-(*   - now intros ????????? H; inv H; constructor. *)
-(*   - now apply external_functions_caller_independent. *)
-(* Qed. *)
-(* Hint Resolve builtin_or_external_caller_independent : caller_independent. *)
 
 (** Combining the semantics given above for the various kinds of external calls,
   we define the predicate [external_call] that relates:
@@ -1769,18 +1750,18 @@ This predicate is used in the semantics of all CompCert languages. *)
 
 Definition external_call (ef: external_function): extcall_sem :=
   match ef with
-  | EF_external cp name sg  => external_functions_sem cp name sg
-  | EF_builtin cp name sg      => builtin_or_external_sem name cp sg
-  | EF_runtime cp name sg      => builtin_or_external_sem name cp sg
-  | EF_vload cp chunk          => volatile_load_sem cp chunk
-  | EF_vstore cp chunk         => volatile_store_sem cp chunk
-  | EF_malloc cp                => extcall_malloc_sem cp
-  | EF_free cp                 => extcall_free_sem cp
-  | EF_memcpy cp sz al         => extcall_memcpy_sem cp sz al
-  | EF_annot cp kind txt targs   => extcall_annot_sem cp txt targs
-  | EF_annot_val cp kind txt targ => extcall_annot_val_sem cp txt targ
-  | EF_inline_asm cp txt sg clb => inline_assembly_sem cp txt sg
-  | EF_debug cp kind txt targs => extcall_debug_sem cp
+  | EF_external name sg  => external_functions_sem name sg
+  | EF_builtin name sg      => builtin_or_external_sem name sg
+  | EF_runtime name sg      => builtin_or_external_sem name sg
+  | EF_vload chunk          => volatile_load_sem chunk
+  | EF_vstore chunk         => volatile_store_sem chunk
+  | EF_malloc                => extcall_malloc_sem
+  | EF_free                 => extcall_free_sem
+  | EF_memcpy sz al         => extcall_memcpy_sem sz al
+  | EF_annot kind txt targs   => extcall_annot_sem txt targs
+  | EF_annot_val kind txt targ => extcall_annot_val_sem txt targ
+  | EF_inline_asm txt sg clb => inline_assembly_sem txt sg
+  | EF_debug kind txt targs => extcall_debug_sem
   end.
 
 Ltac external_call_caller_independent :=
@@ -1832,8 +1813,8 @@ Ltac external_call_caller_independent :=
 (* Qed. *)
 
 Theorem external_call_spec:
-  forall ef,
-  extcall_properties (external_call ef) (comp_of ef) (ef_sig ef).
+  forall ef cp,
+  extcall_properties (external_call ef) cp (ef_sig ef).
 Proof.
   intros. unfold external_call, ef_sig; destruct ef.
   apply external_functions_properties.
@@ -1850,23 +1831,23 @@ Proof.
   apply extcall_debug_ok.
 Qed.
 
-Definition external_call_well_typed_gen ef := ec_well_typed (external_call_spec ef).
-Definition external_call_symbols_preserved ef := ec_symbols_preserved (external_call_spec ef).
-Definition external_call_valid_block ef := ec_valid_block (external_call_spec ef).
-Definition external_call_can_access_block ef := ec_can_access_block (external_call_spec ef).
-Definition external_call_max_perm ef := ec_max_perm (external_call_spec ef).
-Definition external_call_readonly ef := ec_readonly (external_call_spec ef).
-Definition external_call_mem_extends ef := ec_mem_extends (external_call_spec ef).
-Definition external_call_mem_inject_gen ef := ec_mem_inject (external_call_spec ef).
-Definition external_call_trace_length ef := ec_trace_length (external_call_spec ef).
-Definition external_call_receptive ef := ec_receptive (external_call_spec ef).
-Definition external_call_determ ef := ec_determ (external_call_spec ef).
+Definition external_call_well_typed_gen ef cp := ec_well_typed (external_call_spec ef cp).
+Definition external_call_symbols_preserved ef cp := ec_symbols_preserved (external_call_spec ef cp).
+Definition external_call_valid_block ef cp := ec_valid_block (external_call_spec ef cp).
+Definition external_call_can_access_block ef cp := ec_can_access_block (external_call_spec ef cp).
+Definition external_call_max_perm ef cp := ec_max_perm (external_call_spec ef cp).
+Definition external_call_readonly ef cp := ec_readonly (external_call_spec ef cp).
+Definition external_call_mem_extends ef cp := ec_mem_extends (external_call_spec ef cp).
+Definition external_call_mem_inject_gen ef cp := ec_mem_inject (external_call_spec ef cp).
+Definition external_call_trace_length ef cp := ec_trace_length (external_call_spec ef cp).
+Definition external_call_receptive ef cp := ec_receptive (external_call_spec ef cp).
+Definition external_call_determ ef cp := ec_determ (external_call_spec ef cp).
 
 (** Corollary of [external_call_well_typed_gen]. *)
 
 Lemma external_call_well_typed:
-  forall ef ge vargs m1 t vres m2,
-  external_call ef ge vargs m1 t vres m2 ->
+  forall ef ge cp vargs m1 t vres m2,
+  external_call ef ge cp vargs m1 t vres m2 ->
   Val.has_type vres (proj_sig_res (ef_sig ef)).
 Proof.
   intros. apply Val.has_proj_rettype. eapply external_call_well_typed_gen; eauto.
@@ -1875,8 +1856,8 @@ Qed.
 (** Corollary of [external_call_valid_block]. *)
 
 Lemma external_call_nextblock:
-  forall ef ge vargs m1 t vres m2,
-  external_call ef ge vargs m1 t vres m2 ->
+  forall ef ge cp vargs m1 t vres m2,
+  external_call ef ge cp vargs m1 t vres m2 ->
   Ple (Mem.nextblock m1) (Mem.nextblock m2).
 Proof.
   intros. destruct (plt (Mem.nextblock m2) (Mem.nextblock m1)).
@@ -1893,13 +1874,13 @@ Definition meminj_preserves_globals (F V: Type) (ge: Genv.t F V) (f: block -> op
   /\ (forall b1 b2 delta gv, Genv.find_var_info ge b2 = Some gv -> f b1 = Some(b2, delta) -> b2 = b1).
 
 Lemma external_call_mem_inject:
-  forall ef F V (ge: Genv.t F V) vargs m1 t vres m2 f m1' vargs',
+  forall ef F V (ge: Genv.t F V) cp vargs m1 t vres m2 f m1' vargs',
   meminj_preserves_globals ge f ->
-  external_call ef ge vargs m1 t vres m2 ->
+  external_call ef ge cp vargs m1 t vres m2 ->
   Mem.inject f m1 m1' ->
   Val.inject_list f vargs vargs' ->
   exists f', exists vres', exists m2',
-     external_call ef ge vargs' m1' t vres' m2'
+     external_call ef ge cp vargs' m1' t vres' m2'
     /\ Val.inject f' vres vres'
     /\ Mem.inject f' m2 m2'
     /\ Mem.unchanged_on (loc_unmapped f) m1 m2
@@ -1909,7 +1890,7 @@ Lemma external_call_mem_inject:
    /\ (forall b : block,
          ~ Mem.valid_block m1 b ->
          Mem.valid_block m2 b ->
-         exists b' : block, f' b = Some (b', 0) /\ Mem.block_compartment m2 b = Some (comp_of ef)).
+         exists b' : block, f' b = Some (b', 0) /\ Mem.block_compartment m2 b = Some cp).
 Proof.
   intros. destruct H as (A & B & C). eapply external_call_mem_inject_gen with (ge1 := ge); eauto.
   repeat split; intros.
@@ -1926,18 +1907,18 @@ Qed.
 (** Corollaries of [external_call_determ]. *)
 
 Lemma external_call_match_traces:
-  forall ef ge vargs m t1 vres1 m1 t2 vres2 m2,
-  external_call ef ge vargs m t1 vres1 m1 ->
-  external_call ef ge vargs m t2 vres2 m2 ->
+  forall ef ge cp vargs m t1 vres1 m1 t2 vres2 m2,
+  external_call ef ge cp vargs m t1 vres1 m1 ->
+  external_call ef ge cp vargs m t2 vres2 m2 ->
   match_traces ge t1 t2.
 Proof.
   intros. exploit external_call_determ. eexact H. eexact H0. tauto.
 Qed.
 
 Lemma external_call_deterministic:
-  forall ef ge vargs m t vres1 m1 vres2 m2,
-  external_call ef ge vargs m t vres1 m1 ->
-  external_call ef ge vargs m t vres2 m2 ->
+  forall ef ge cp vargs m t vres1 m1 vres2 m2,
+  external_call ef ge cp vargs m t vres1 m1 ->
+  external_call ef ge cp vargs m t vres2 m2 ->
   vres1 = vres2 /\ m1 = m2.
 Proof.
   intros. exploit external_call_determ. eexact H. eexact H0. intuition.
@@ -1949,6 +1930,7 @@ Section EVAL_BUILTIN_ARG.
 
 Variable A: Type.
 Variable ge: Senv.t.
+Variable cp: compartment.
 Variable e: A -> val.
 Variable sp: val.
 Variable m: mem.
